removed an assume

examples/low-level/crypto/Crypto.Symmetric.Poly1305.Spec.fst
@@ -66,7 +66,14 @@ let encode (w:word) : Tot elem =
   pow2_le_compat 128 (8 * l);
   pow2 (8 * l) +@ little_endian w
 
-private assume val lemma_encode_nonzero: v:word_16 -> Lemma (encode v <> 0)
+val lemma_encode_nonzero: v:word_16 -> Lemma (encode v <> 0)
+let lemma_encode_nonzero v =
+  lemma_little_endian_is_bounded v;
+  Math.Lemmas.pow2_double_sum 128;
+  cut (pow2 (8 * length v) + little_endian v < pow2 129);
+  assert_norm(pow2 129 < pow2 130 - 5);
+  Math.Lemmas.modulo_lemma (pow2 (8 * length v) + little_endian v) p_1305
+
 
 let trunc_1305 (e:elem) : Tot elem = e % pow2 128
 
